messageInvariantPrototypes/toyLeaderElection/withoutMonotonic/messageInvariants.dfy
@@ -3,30 +3,34 @@ include "spec.dfy"
 module MessageInvariants {
 import opened Types
 import opened UtilitiesLibrary
+import Host
 import opened DistributedSystem
 
 // Message Invariant: self inductive
-predicate ValidMessages(c: Constants, v: Variables) 
+// Property of send
+predicate ValidMessageSource(c: Constants, v: Variables) 
   requires v.WF(c)
 {
   forall msg | msg in v.network.sentMsgs 
   :: match msg 
       case VoteReq(candidate) => c.ValidIdx(candidate)
-      case Vote(voter, candidate) => c.ValidIdx(voter) && c.ValidIdx(candidate)
+      case Vote(voter, candidate) => c.ValidIdx(voter)
       case Leader(src) => c.ValidIdx(src)
       case _ => true
 }
 
 // Message Invariant: self inductive
+// Property of Send
 predicate LeaderMsgImpliesLocalQuorum(c: Constants, v: Variables) 
   requires v.WF(c)
-  requires ValidMessages(c, v)
+  requires ValidMessageSource(c, v)
 {
   forall msg | msg in v.network.sentMsgs && msg.Leader?
   :: SetIsQuorum(c.hostConstants[msg.src].clusterSize, v.hosts[msg.src].receivedVotes)
 }
 
 // Message Invariant: self inductive
+// Property of Receive
 predicate ReceivedVotesValidity(c: Constants, v: Variables) 
   requires v.WF(c)
 {
@@ -35,9 +39,10 @@ predicate ReceivedVotesValidity(c: Constants, v: Variables)
 }
 
 // Message Invariant: self inductive
+// Property of Send
 predicate VoteMsgImpliesVoterVoted(c: Constants, v: Variables)
   requires v.WF(c)
-  requires ValidMessages(c, v)
+  requires ValidMessageSource(c, v)
 {
   forall msg | msg in v.network.sentMsgs && msg.Vote?
   :: v.hosts[msg.voter].voted
@@ -46,7 +51,7 @@ predicate VoteMsgImpliesVoterVoted(c: Constants, v: Variables)
 predicate MessageInv(c: Constants, v: Variables) 
 {
   && v.WF(c)
-  && ValidMessages(c, v)
+  && ValidMessageSource(c, v)
   && LeaderMsgImpliesLocalQuorum(c, v)
   && ReceivedVotesValidity(c, v)
   && VoteMsgImpliesVoterVoted(c, v)
@@ -61,6 +66,35 @@ lemma MessageInvInductive(c: Constants, v: Variables, v': Variables)
   requires MessageInv(c, v)
   requires Next(c, v, v')
   ensures MessageInv(c, v')
-{}
+{
+  InvNextLeaderMsgImpliesLocalQuorum(c, v, v');
+}
+
+
+/***************************************************************************************
+*                               Proofs (how unfortunate)                               *
+***************************************************************************************/
+
+lemma InvNextLeaderMsgImpliesLocalQuorum(c: Constants, v: Variables, v': Variables)
+  requires v.WF(c)
+  requires ValidMessageSource(c, v)
+  requires LeaderMsgImpliesLocalQuorum(c, v)
+  requires Next(c, v, v')
+  ensures LeaderMsgImpliesLocalQuorum(c, v')
+{
+  forall msg | msg in v'.network.sentMsgs && msg.Leader?
+  ensures SetIsQuorum(c.hostConstants[msg.src].clusterSize, v'.hosts[msg.src].receivedVotes)
+  {
+    var dsStep :| NextStep(c, v, v', dsStep);
+    var actor, msgOps := dsStep.actorIdx, dsStep.msgOps;
+    var step :| Host.NextStep(c.hostConstants[actor], v.hosts[actor], v'.hosts[actor], step, msgOps);
+    if !step.VictoryStep? {
+      assert msg in v.network.sentMsgs;  // trigger
+      assert SetIsQuorum(c.hostConstants[msg.src].clusterSize, v'.hosts[msg.src].receivedVotes); // trigger
+    }
+  }
+}
+
+
 }
 
